Word256Auxiliary.thy
@@ -19,15 +19,14 @@ begin
 
 lemma bs_to_w256_def_lemma:
 " ((\<forall> seq.
-   (case  resizeBitSeq (Some (( 256 :: nat))) seq of
-         BitSeq _ s b => W256 s b
-   ) = (\<lambda> w .  word_of_int (integerFromBitSeq w)) seq)) "
+   W256 (integerFromBitSeq seq) =
+     (\<lambda> w .  word_of_int (integerFromBitSeq w)) seq)) "
 (* Theorem: bs_to_w256_def_lemma*)(* try *) by auto
 
 lemma w256_to_bs_def_lemma:
-" ((\<forall> s. \<forall> b.
-   BitSeq (Some (( 256 :: nat))) s b =
-     (\<lambda> w .  bitSeqFromInteger (Some 256) ( (sint w))) (W256 s b))) "
+" ((\<forall> i.
+   bitSeqFromInteger (Some (( 256 :: nat))) i =
+     (\<lambda> w .  bitSeqFromInteger (Some 256) ( (sint w))) (W256 i))) "
 (* Theorem: w256_to_bs_def_lemma*)(* try *) by auto
 
 lemma word256ToNat_def_lemma:
@@ -49,16 +48,11 @@ lemma word256ToInt_def_lemma:
 (* Theorem: word256ToInt_def_lemma*)(* try *) by auto
 
 lemma word256FromInteger_def_lemma:
-" ((\<forall> i.
-   (\<lambda> w .  word_of_int (integerFromBitSeq w))
-     (bitSeqFromInteger (Some (( 256 :: nat))) i) =
-     (\<lambda> i .  word_of_int ( i)) i)) "
+" ((\<forall> i. W256 (i mod base) = (\<lambda> i .  word_of_int ( i)) i)) "
 (* Theorem: word256FromInteger_def_lemma*)(* try *) by auto
 
 lemma word256FromInt_def_lemma:
-" ((\<forall> i.
-   (\<lambda> w .  word_of_int (integerFromBitSeq w))
-     (bitSeqFromInteger (Some (( 256 :: nat))) ( i)) = word_of_int i)) "
+" ((\<forall> i. W256 ( i mod base) = word_of_int i)) "
 (* Theorem: word256FromInt_def_lemma*)(* try *) by auto
 
 lemma word256FromBoollist_def_lemma:
@@ -74,116 +68,118 @@ lemma boolListFromWord256_def_lemma:
 " ((\<forall> w.
    boolListFrombitSeq (( 256 :: nat))
      ((\<lambda> w .  bitSeqFromInteger (Some 256) ( (sint w))) w) = 
-   of_bl w)) "
+   to_bl w)) "
 (* Theorem: boolListFromWord256_def_lemma*)(* try *) by auto
 
 lemma word256FromNumeral_def_lemma:
-" ((\<forall> w.
-   (\<lambda> w .  word_of_int (integerFromBitSeq w))
-     (bitSeqFromInteger None (( w :: int))) = ((word_of_int w) :: 256 word))) "
+" ((\<forall> w. W256 (( w :: int) mod base) = ((word_of_int w) :: 256 word))) "
 (* Theorem: word256FromNumeral_def_lemma*)(* try *) by auto
 
 lemma w256Less_def_lemma:
 " ((\<forall> bs1. \<forall> bs2.
-   word256BinTest bitSeqLess bs1 bs2 = word_sless bs1 bs2)) "
+   word256BinTest (op<) bs1 bs2 = word_sless bs1 bs2)) "
 (* Theorem: w256Less_def_lemma*)(* try *) by auto
 
 lemma w256LessEqual_def_lemma:
 " ((\<forall> bs1. \<forall> bs2.
-   word256BinTest bitSeqLessEqual bs1 bs2 = word_sle bs1 bs2)) "
+   word256BinTest (op \<le>) bs1 bs2 = word_sle bs1 bs2)) "
 (* Theorem: w256LessEqual_def_lemma*)(* try *) by auto
 
 lemma w256Greater_def_lemma:
 " ((\<forall> bs1. \<forall> bs2.
-   word256BinTest bitSeqGreater bs1 bs2 = word_sless bs2 bs1)) "
+   word256BinTest (op>) bs1 bs2 = word_sless bs2 bs1)) "
 (* Theorem: w256Greater_def_lemma*)(* try *) by auto
 
 lemma w256GreaterEqual_def_lemma:
 " ((\<forall> bs1. \<forall> bs2.
-   word256BinTest bitSeqGreaterEqual bs1 bs2 = word_sle bs2 bs1)) "
+   word256BinTest (op \<ge>) bs1 bs2 = word_sle bs2 bs1)) "
 (* Theorem: w256GreaterEqual_def_lemma*)(* try *) by auto
 
 lemma w256Compare_def_lemma:
 " ((\<forall> bs1. \<forall> bs2.
-   word256BinTest bitSeqCompare bs1 bs2 =
+   word256BinTest (genericCompare (op<) (op=)) bs1 bs2 =
      (genericCompare word_sless w256Eq bs1 bs2))) "
 (* Theorem: w256Compare_def_lemma*)(* try *) by auto
 
 lemma word256Negate_def_lemma:
-" (( word256UnaryOp bitSeqNegate = (\<lambda> i. - i))) "
+" (( word256UnaryOp (\<lambda> i. - i) = (\<lambda> i. - i))) "
 (* Theorem: word256Negate_def_lemma*)(* try *) by auto
 
 lemma word256Succ_def_lemma:
-" (( word256UnaryOp bitSeqSucc = (\<lambda> n. n + 1))) "
+" (( word256UnaryOp (\<lambda> n. n + ( 1 :: int)) = (\<lambda> n. n + 1))) "
 (* Theorem: word256Succ_def_lemma*)(* try *) by auto
 
 lemma word256Pred_def_lemma:
-" (( word256UnaryOp bitSeqPred = (\<lambda> n. n - 1))) "
+" (( word256UnaryOp (\<lambda> n. n - ( 1 :: int)) = (\<lambda> n. n - 1))) "
 (* Theorem: word256Pred_def_lemma*)(* try *) by auto
 
 lemma word256Lnot_def_lemma:
-" (( word256UnaryOp bitSeqNot = (\<lambda> w. (NOT w)))) "
+" (( word256UnaryOp integerLnot = (\<lambda> w. (NOT w)))) "
 (* Theorem: word256Lnot_def_lemma*)(* try *) by auto
 
 lemma word256Add_def_lemma:
-" (( word256BinOp bitSeqAdd = (op+))) "
+" (( word256BinOp (op+) = (op+))) "
 (* Theorem: word256Add_def_lemma*)(* try *) by auto
 
 lemma word256Minus_def_lemma:
-" (( word256BinOp bitSeqMinus = (op-))) "
+" (( word256BinOp (op-) = (op-))) "
 (* Theorem: word256Minus_def_lemma*)(* try *) by auto
 
 lemma word256Mult_def_lemma:
-" (( word256BinOp bitSeqMult = (op*))) "
+" (( word256BinOp (op*) = (op*))) "
 (* Theorem: word256Mult_def_lemma*)(* try *) by auto
 
 lemma word256IntegerDivision_def_lemma:
-" (( word256BinOp bitSeqDiv = (op div))) "
+" (( word256BinOp (op div) = (op div))) "
 (* Theorem: word256IntegerDivision_def_lemma*)(* try *) by auto
 
 lemma word256Division_def_lemma:
-" (( word256BinOp bitSeqDiv = (op div))) "
+" (( word256BinOp (op div) = (op div))) "
 (* Theorem: word256Division_def_lemma*)(* try *) by auto
 
 lemma word256Remainder_def_lemma:
-" (( word256BinOp bitSeqMod = (op mod))) "
+" (( word256BinOp (op mod) = (op mod))) "
 (* Theorem: word256Remainder_def_lemma*)(* try *) by auto
 
 lemma word256Land_def_lemma:
-" (( word256BinOp bitSeqAnd = (op AND))) "
+" (( word256BinOp integerLand = (op AND))) "
 (* Theorem: word256Land_def_lemma*)(* try *) by auto
 
 lemma word256Lor_def_lemma:
-" (( word256BinOp bitSeqOr = (op OR))) "
+" (( word256BinOp integerLor = (op OR))) "
 (* Theorem: word256Lor_def_lemma*)(* try *) by auto
 
 lemma word256Lxor_def_lemma:
-" (( word256BinOp bitSeqXor = (op XOR))) "
+" (( word256BinOp integerLxor = (op XOR))) "
 (* Theorem: word256Lxor_def_lemma*)(* try *) by auto
 
 lemma word256Min_def_lemma:
-" (( word256BinOp (bitSeqMin) = min)) "
+" (( word256BinOp (min) = min)) "
 (* Theorem: word256Min_def_lemma*)(* try *) by auto
 
 lemma word256Max_def_lemma:
-" (( word256BinOp (bitSeqMax) = max)) "
+" (( word256BinOp (max) = max)) "
 (* Theorem: word256Max_def_lemma*)(* try *) by auto
 
 lemma word256Power_def_lemma:
-" (( word256NatOp bitSeqPow = (op^))) "
+" (( word256NatOp (op^) = (op^))) "
 (* Theorem: word256Power_def_lemma*)(* try *) by auto
 
 lemma word256Asr_def_lemma:
-" (( word256NatOp bitSeqArithmeticShiftRight = (op>>>))) "
+" (( word256NatOp integerAsr = (op>>>))) "
 (* Theorem: word256Asr_def_lemma*)(* try *) by auto
 
 lemma word256Lsr_def_lemma:
-" (( word256NatOp bitSeqLogicalShiftRight = (op>>))) "
+" (( word256NatOp integerAsr = (op>>))) "
 (* Theorem: word256Lsr_def_lemma*)(* try *) by auto
 
 lemma word256Lsl_def_lemma:
-" (( word256NatOp bitSeqShiftLeft = (op<<))) "
+" (( word256NatOp integerLsl = (op<<))) "
 (* Theorem: word256Lsl_def_lemma*)(* try *) by auto
+
+lemma word256UGT_def_lemma:
+" ((\<forall> a. \<forall> b. (unat a > unat b) = a > b)) "
+(* Theorem: word256UGT_def_lemma*)(* try *) by auto
 
 
 
